clk added to events + commutes fixed + causal_dep partial order defined

txn-data-consistency/EP+.thy
@@ -193,44 +193,58 @@ abbreviation is_done_w :: "('v, 'm) global_conf_scheme \<Rightarrow> txid \<Righ
 subsection \<open>Events\<close>
 
 datatype 'v ev =
-  RInvoke cl_id "key set" sqn | Read cl_id key 'v txid tstmp tstmp sqn | RDone cl_id "key \<rightharpoonup> 'v" sqn view |
-  WInvoke cl_id "key \<rightharpoonup> 'v" sqn | WCommit cl_id "key \<rightharpoonup> 'v" tstmp sqn view | WDone cl_id "key \<rightharpoonup> 'v" sqn |
-  RegR key txid0 txid tstmp | PrepW key txid0 'v | CommitW key txid0 'v tstmp | Skip2
+  RInvoke cl_id "key set" sqn tstmp | Read cl_id key 'v txid tstmp tstmp sqn tstmp
+  | RDone cl_id "key \<rightharpoonup> 'v" sqn view tstmp | WInvoke cl_id "key \<rightharpoonup> 'v" sqn tstmp
+  | WCommit cl_id "key \<rightharpoonup> 'v" tstmp sqn view tstmp | WDone cl_id "key \<rightharpoonup> 'v" sqn tstmp
+  | RegR key txid0 txid tstmp tstmp | PrepW key txid0 'v tstmp | CommitW key txid0 'v tstmp tstmp
+  | Skip2
 
 fun commit_ev :: "'v ev \<Rightarrow> bool" where
-  "commit_ev (RDone cl kv_map sn u'') = True" |
-  "commit_ev (WCommit cl kv_map cts sn u'') = True" |
+  "commit_ev (RDone cl kv_map sn u'' clk) = True" |
+  "commit_ev (WCommit cl kv_map cts sn u'' clk) = True" |
   "commit_ev _ = False"
 
 fun ev_cl :: "'v ev \<Rightarrow> cl_id" where
-  "ev_cl (RInvoke cl keys sn)           = cl" |
-  "ev_cl (Read cl k v t rts rlst sn)    = cl" |
-  "ev_cl (RDone cl kv_map sn u'')       = cl" |
-  "ev_cl (WInvoke cl kv_map sn)         = cl" |
-  "ev_cl (WCommit cl kv_map cts sn u'') = cl" |
-  "ev_cl (WDone cl kv_map sn)           = cl" |
-  "ev_cl (RegR svr t t_wr rts)          = get_cl t" |
-  "ev_cl (PrepW svr t v)                = get_cl t" |
-  "ev_cl (CommitW svr t v cts)          = get_cl t" |
-  "ev_cl Skip2                          = 0" \<comment> \<open>dummy value\<close>
+  "ev_cl (RInvoke cl keys sn clk)           = cl" |
+  "ev_cl (Read cl k v t rts rlst sn clk)    = cl" |
+  "ev_cl (RDone cl kv_map sn u'' clk)       = cl" |
+  "ev_cl (WInvoke cl kv_map sn clk)         = cl" |
+  "ev_cl (WCommit cl kv_map cts sn u'' clk) = cl" |
+  "ev_cl (WDone cl kv_map sn clk)           = cl" |
+  "ev_cl (RegR svr t t_wr rts clk)          = get_cl t" |
+  "ev_cl (PrepW svr t v clk)                = get_cl t" |
+  "ev_cl (CommitW svr t v cts clk)          = get_cl t" |
+  "ev_cl Skip2                              = 0" \<comment> \<open>dummy value\<close>
 
 fun ev_key :: "'v ev \<Rightarrow> key option" where
-  "ev_key (RegR svr t t_wr rts)         = Some svr" |
-  "ev_key (PrepW svr t v)               = Some svr" |
-  "ev_key (CommitW svr t v cts)         = Some svr" |
+  "ev_key (RegR svr t t_wr rts clk)         = Some svr" |
+  "ev_key (PrepW svr t v clk)               = Some svr" |
+  "ev_key (CommitW svr t v cts clk)         = Some svr" |
   "ev_key _ = None"
 
 fun ev_txn :: "'v ev \<Rightarrow> txid" where
-  "ev_txn (RInvoke cl keys sn)           = Tn (Tn_cl sn cl)" |
-  "ev_txn (Read cl k v t rts rlst sn)    = Tn (Tn_cl sn cl)" |
-  "ev_txn (RDone cl kv_map sn u'')       = Tn (Tn_cl sn cl)" |
-  "ev_txn (WInvoke cl kv_map sn)         = Tn (Tn_cl sn cl)" |
-  "ev_txn (WCommit cl kv_map cts sn u'') = Tn (Tn_cl sn cl)" |
-  "ev_txn (WDone cl kv_map sn)           = Tn (Tn_cl sn cl)" |
-  "ev_txn (RegR svr t t_wr rts)          = Tn t" |
-  "ev_txn (PrepW svr t v)                = Tn t" |
-  "ev_txn (CommitW svr t v cts)          = Tn t" |
-  "ev_txn Skip2                          = T0" \<comment> \<open>dummy value\<close>
+  "ev_txn (RInvoke cl keys sn clk)           = Tn (Tn_cl sn cl)" |
+  "ev_txn (Read cl k v t rts rlst sn clk)    = Tn (Tn_cl sn cl)" |
+  "ev_txn (RDone cl kv_map sn u'' clk)       = Tn (Tn_cl sn cl)" |
+  "ev_txn (WInvoke cl kv_map sn clk)         = Tn (Tn_cl sn cl)" |
+  "ev_txn (WCommit cl kv_map cts sn u'' clk) = Tn (Tn_cl sn cl)" |
+  "ev_txn (WDone cl kv_map sn clk)           = Tn (Tn_cl sn cl)" |
+  "ev_txn (RegR svr t t_wr rts clk)          = Tn t" |
+  "ev_txn (PrepW svr t v clk)                = Tn t" |
+  "ev_txn (CommitW svr t v cts clk)          = Tn t" |
+  "ev_txn Skip2                              = T0" \<comment> \<open>dummy value\<close>
+
+fun ev_clk :: "'v ev \<Rightarrow> tstmp" where
+  "ev_clk (RInvoke cl keys sn clk)           = clk" |
+  "ev_clk (Read cl k v t rts rlst sn clk)    = clk" |
+  "ev_clk (RDone cl kv_map sn u'' clk)       = clk" |
+  "ev_clk (WInvoke cl kv_map sn clk)         = clk" |
+  "ev_clk (WCommit cl kv_map cts sn u'' clk) = clk" |
+  "ev_clk (WDone cl kv_map sn clk)           = clk" |
+  "ev_clk (RegR svr t t_wr rts clk)          = clk" |
+  "ev_clk (PrepW svr t v clk)                = clk" |
+  "ev_clk (CommitW svr t v cts clk)          = clk" |
+  "ev_clk Skip2                              = 0" \<comment> \<open>dummy value\<close>
 
 definition ects :: "tstmp \<Rightarrow> cl_id \<Rightarrow> tstmp \<times> cl_id" where
   "ects cts cl = (cts, Suc cl)"
@@ -241,12 +255,12 @@ lemma ects_inj: "ects cts cl = ects cts' cl' \<Longrightarrow> cts = cts' \<and>
 lemma min_ects: "(0, 0) < ects x y" by (auto simp add: less_prod_def ects_def)
 
 fun ev_ects :: "'v ev \<Rightarrow> (tstmp \<times> cl_id) option" where
-  "ev_ects (WCommit cl kv_map cts sn u'') = Some (ects cts cl)" |
+  "ev_ects (WCommit cl kv_map cts sn u'' clk) = Some (ects cts cl)" |
   "ev_ects _ = None"
 
 lemma ev_ects_Some:
   "ev_ects e = Some (cts, Suc_cl)
-  \<Longrightarrow> \<exists>cl kv_map sn u''. e = WCommit cl kv_map cts sn u'' \<and> Suc_cl = Suc cl"
+  \<Longrightarrow> \<exists>cl kv_map sn u'' clk. e = WCommit cl kv_map cts sn u'' clk \<and> Suc_cl = Suc cl"
   by (cases e, simp_all add: ects_def)
 
 definition unique_ts :: "(txid \<rightharpoonup> tstmp) \<Rightarrow> txid \<Rightarrow> tstmp \<times> cl_id" where
@@ -261,10 +275,11 @@ lemma unique_ts_def':
 subsubsection \<open>Client Events\<close>
 
 definition read_invoke_G where
-  "read_invoke_G cl keys sn s \<equiv>
+  "read_invoke_G cl keys sn clk s \<equiv>
     keys \<noteq> {} \<and>
     finite keys \<and>
     sn = cl_sn (cls s cl) \<and>
+    clk = Suc (cl_clock (cls s cl)) \<and>
     cl_state (cls s cl) = Idle"
 
 definition read_invoke_U where
@@ -277,17 +292,18 @@ definition read_invoke_U where
       \<rparr>)
     \<rparr>"
 
-definition read_invoke :: "cl_id \<Rightarrow> key set \<Rightarrow> sqn \<Rightarrow> ('v, 'm) global_conf_scheme \<Rightarrow> ('v, 'm) global_conf_scheme \<Rightarrow> bool" where
-  "read_invoke cl keys sn s s' \<equiv>
-    read_invoke_G cl keys sn s \<and>
+definition read_invoke :: "cl_id \<Rightarrow> key set \<Rightarrow> sqn \<Rightarrow> tstmp \<Rightarrow> ('v, 'm) global_conf_scheme \<Rightarrow> ('v, 'm) global_conf_scheme \<Rightarrow> bool" where
+  "read_invoke cl keys sn clk s s' \<equiv>
+    read_invoke_G cl keys sn clk s \<and>
     s' = read_invoke_U cl keys s"
 
 definition read_G where
-  "read_G cl k v t rts rlst sn s \<equiv> 
+  "read_G cl k v t rts rlst sn clk s \<equiv> 
     \<comment> \<open>reads server k's value v for client transaction, lst, and svr_clock\<close>
     (\<exists>cts ts lst rs. svr_state (svrs s k) t = Commit cts ts lst v rs \<and> (get_txn s cl, rts, rlst) \<in> rs) \<and>
     (\<exists>keys kv_map. cl_state (cls s cl) = RtxnInProg keys kv_map \<and> k \<in> keys \<and> kv_map k = None) \<and>
-    sn = cl_sn (cls s cl)"
+    sn = cl_sn (cls s cl) \<and>
+    clk = Suc (max (cl_clock (cls s cl)) rts)"
 
 definition read_U where
   "read_U cl k v rts rlst s \<equiv>
@@ -300,14 +316,15 @@ definition read_U where
       \<rparr>)
     \<rparr>"
 
-definition read :: "cl_id \<Rightarrow> key \<Rightarrow> 'v \<Rightarrow> txid \<Rightarrow> tstmp \<Rightarrow> tstmp \<Rightarrow> sqn \<Rightarrow> ('v, 'm) global_conf_scheme \<Rightarrow> ('v, 'm) global_conf_scheme \<Rightarrow> bool" where
-  "read cl k v t rts rlst sn s s' \<equiv>
-    read_G cl k v t rts rlst sn s \<and>
+definition read :: "cl_id \<Rightarrow> key \<Rightarrow> 'v \<Rightarrow> txid \<Rightarrow> tstmp \<Rightarrow> tstmp \<Rightarrow> sqn \<Rightarrow> tstmp \<Rightarrow> ('v, 'm) global_conf_scheme \<Rightarrow> ('v, 'm) global_conf_scheme \<Rightarrow> bool" where
+  "read cl k v t rts rlst sn clk s s' \<equiv>
+    read_G cl k v t rts rlst sn clk s \<and>
     s' = read_U cl k v rts rlst s"
 
 definition read_done_G where
-  "read_done_G cl kv_map sn s \<equiv>
+  "read_done_G cl kv_map sn clk s \<equiv>
     sn = cl_sn (cls s cl) \<and>
+    clk = Suc (cl_clock (cls s cl)) \<and>
     cl_state (cls s cl) = RtxnInProg (dom kv_map) kv_map"
 
 definition read_done_U where
@@ -322,16 +339,17 @@ definition read_done_U where
       rtxn_rts := (rtxn_rts s) (get_txn s cl \<mapsto> gst (cls s cl))
     \<rparr>"
 
-definition read_done :: "cl_id \<Rightarrow> (key \<rightharpoonup> 'v) \<Rightarrow> sqn \<Rightarrow> view \<Rightarrow> ('v, 'm) global_conf_scheme \<Rightarrow> ('v, 'm) global_conf_scheme \<Rightarrow> bool" where
-  "read_done cl kv_map sn u'' s s' \<equiv>
-    read_done_G cl kv_map sn s \<and>
+definition read_done :: "cl_id \<Rightarrow> (key \<rightharpoonup> 'v) \<Rightarrow> sqn \<Rightarrow> view \<Rightarrow> tstmp \<Rightarrow> ('v, 'm) global_conf_scheme \<Rightarrow> ('v, 'm) global_conf_scheme \<Rightarrow> bool" where
+  "read_done cl kv_map sn u'' clk s s' \<equiv>
+    read_done_G cl kv_map sn clk s \<and>
     s' = read_done_U cl kv_map s"
 
 definition write_invoke_G where
-  "write_invoke_G cl kv_map sn s \<equiv> 
+  "write_invoke_G cl kv_map sn clk s \<equiv> 
     kv_map \<noteq> Map.empty \<and>
     finite (dom kv_map) \<and>
     sn = cl_sn (cls s cl) \<and>
+    clk = Suc (cl_clock (cls s cl)) \<and>
     cl_state (cls s cl) = Idle"
 
 definition write_invoke_U where
@@ -343,14 +361,15 @@ definition write_invoke_U where
       \<rparr>)
     \<rparr>"
 
-definition write_invoke :: "cl_id \<Rightarrow> (key \<rightharpoonup> 'v) \<Rightarrow> sqn \<Rightarrow> ('v, 'm) global_conf_scheme \<Rightarrow> ('v, 'm) global_conf_scheme \<Rightarrow> bool" where
-  "write_invoke cl kv_map sn s s' \<equiv> 
-    write_invoke_G cl kv_map sn s \<and>
+definition write_invoke :: "cl_id \<Rightarrow> (key \<rightharpoonup> 'v) \<Rightarrow> sqn \<Rightarrow> tstmp \<Rightarrow> ('v, 'm) global_conf_scheme \<Rightarrow> ('v, 'm) global_conf_scheme \<Rightarrow> bool" where
+  "write_invoke cl kv_map sn clk s s' \<equiv> 
+    write_invoke_G cl kv_map sn clk s \<and>
     s' = write_invoke_U cl kv_map s"
 
 definition write_commit_G where
-  "write_commit_G cl kv_map cts sn s \<equiv>
+  "write_commit_G cl kv_map cts sn clk s \<equiv>
     sn = cl_sn (cls s cl) \<and>            \<comment> \<open>@{term sn} needed in mediator function, not in event\<close>
+    clk = Suc (max (cl_clock (cls s cl)) cts) \<and>
     cl_state (cls s cl) = WtxnPrep kv_map \<and>
     (\<forall>k \<in> dom kv_map. \<exists>ts v. svr_state (svrs s k) (get_wtxn s cl) = Prep ts v \<and> kv_map k = Some v) \<and>
     cts = Max {get_ts (svr_state (svrs s k) (get_wtxn s cl)) | k. k \<in> dom kv_map}"
@@ -369,17 +388,23 @@ definition write_commit_U where
         (unique_ts ((wtxn_cts s) (get_wtxn s cl \<mapsto> cts))) (cts_order s)
     \<rparr>"
 
-definition write_commit :: "cl_id \<Rightarrow> (key \<rightharpoonup> 'v) \<Rightarrow> tstmp \<Rightarrow> sqn \<Rightarrow> view \<Rightarrow> ('v, 'm) global_conf_scheme \<Rightarrow> ('v, 'm) global_conf_scheme \<Rightarrow> bool" where
-  "write_commit cl kv_map cts sn u'' s s' \<equiv>
-    write_commit_G cl kv_map cts sn s \<and> 
+definition write_commit :: "cl_id \<Rightarrow> (key \<rightharpoonup> 'v) \<Rightarrow> tstmp \<Rightarrow> sqn \<Rightarrow> view \<Rightarrow> tstmp \<Rightarrow> ('v, 'm) global_conf_scheme \<Rightarrow> ('v, 'm) global_conf_scheme \<Rightarrow> bool" where
+  "write_commit cl kv_map cts sn u'' clk s s' \<equiv>
+    write_commit_G cl kv_map cts sn clk s \<and> 
     s' = write_commit_U cl kv_map cts s"
 
+definition clk_WDone where
+  "clk_WDone cl kv_map clk s \<equiv> clk =
+        Suc (max (cl_clock (cls s cl))
+              (Max {get_sclk (svr_state (svrs s k) (get_wtxn s cl)) |k. k \<in> dom kv_map}))"
+
 definition write_done_G where
-  "write_done_G cl kv_map sn s \<equiv>
+  "write_done_G cl kv_map sn clk s \<equiv>
     (\<exists>cts. cl_state (cls s cl) = WtxnCommit cts kv_map \<and>
       (\<forall>k\<in>dom kv_map. \<exists>ts lst v rs. svr_state (svrs s k) (get_wtxn s cl) = Commit cts ts lst v rs \<and>
          kv_map k = Some v)) \<and>
-    sn = cl_sn (cls s cl)"
+    sn = cl_sn (cls s cl) \<and>
+    clk_WDone cl kv_map clk s"
 
 definition write_done_U where
   "write_done_U cl kv_map s \<equiv>
@@ -387,14 +412,15 @@ definition write_done_U where
       (cl := cls s cl \<lparr>
         cl_state := Idle,
         cl_sn := Suc (cl_sn (cls s cl)),
-        cl_clock := Suc (max (cl_clock (cls s cl)) (Max {get_sclk (svr_state (svrs s k) (get_wtxn s cl)) | k. k \<in> dom kv_map})),
+        cl_clock := Suc (max (cl_clock (cls s cl))
+              (Max {get_sclk (svr_state (svrs s k) (get_wtxn s cl)) |k. k \<in> dom kv_map})),
         lst_map := (\<lambda>k. if kv_map k = None then lst_map (cls s cl) k else get_lst (svr_state (svrs s k) (get_wtxn s cl)))
       \<rparr>)
     \<rparr>"
 
-definition write_done :: "cl_id \<Rightarrow> (key \<rightharpoonup> 'v) \<Rightarrow> sqn \<Rightarrow> ('v, 'm) global_conf_scheme \<Rightarrow> ('v, 'm) global_conf_scheme \<Rightarrow> bool" where
-  "write_done cl kv_map sn s s' \<equiv>
-    write_done_G cl kv_map sn s \<and>
+definition write_done :: "cl_id \<Rightarrow> (key \<rightharpoonup> 'v) \<Rightarrow> sqn \<Rightarrow> tstmp \<Rightarrow> ('v, 'm) global_conf_scheme \<Rightarrow> ('v, 'm) global_conf_scheme \<Rightarrow> bool" where
+  "write_done cl kv_map sn clk s s' \<equiv>
+    write_done_G cl kv_map sn clk s \<and>
     s' = write_done_U cl kv_map s"
 
 
@@ -408,10 +434,11 @@ definition write_done :: "cl_id \<Rightarrow> (key \<rightharpoonup> 'v) \<Right
 subsubsection \<open>Server Events\<close>
 
 definition register_read_G where
-  "register_read_G svr t t_wr rts s \<equiv>
+  "register_read_G svr t t_wr rts clk s \<equiv>
     is_curr_t s t \<and>
     (\<exists>keys kv_map. cl_state (cls s (get_cl t)) = RtxnInProg keys kv_map \<and> svr \<in> keys \<and> kv_map svr = None) \<and>
     rts = gst (cls s (get_cl t)) \<and>
+    clk = Suc (max (svr_clock (svrs s svr)) (cl_clock (cls s (get_cl t)))) \<and>
     t_wr = read_at (svr_state (svrs s svr)) rts (get_cl t)"
 
 definition register_read_U where
@@ -423,14 +450,15 @@ definition register_read_U where
       \<rparr>)
     \<rparr>"
 
-definition register_read :: "key \<Rightarrow> txid0 \<Rightarrow> txid \<Rightarrow> tstmp \<Rightarrow> ('v, 'm) global_conf_scheme \<Rightarrow> ('v, 'm) global_conf_scheme \<Rightarrow> bool" where
-  "register_read svr t t_wr rts s s' \<equiv>
-    register_read_G svr t t_wr rts s \<and>
+definition register_read :: "key \<Rightarrow> txid0 \<Rightarrow> txid \<Rightarrow> tstmp \<Rightarrow> tstmp \<Rightarrow> ('v, 'm) global_conf_scheme \<Rightarrow> ('v, 'm) global_conf_scheme \<Rightarrow> bool" where
+  "register_read svr t t_wr rts clk s s' \<equiv>
+    register_read_G svr t t_wr rts clk s \<and>
     s' = register_read_U svr t t_wr s"
 
 definition prepare_write_G where
-  "prepare_write_G svr t v s \<equiv>
+  "prepare_write_G svr t v clk s \<equiv>
     is_curr_t s t \<and>
+    clk = Suc (max (svr_clock (svrs s svr)) (cl_clock (cls s (get_cl t)))) \<and>
     \<comment> \<open>get client's value v for svr and cl_clock\<close>
     (\<exists>kv_map. cl_state (cls s (get_cl t)) = WtxnPrep kv_map \<and> kv_map svr = Some v) \<and>
     svr_state (svrs s svr) (Tn t) = No_Ver"
@@ -444,14 +472,15 @@ definition prepare_write_U where
       \<rparr>)
     \<rparr>"
 
-definition prepare_write :: "key \<Rightarrow> txid0 \<Rightarrow> 'v \<Rightarrow> ('v, 'm) global_conf_scheme \<Rightarrow> ('v, 'm) global_conf_scheme \<Rightarrow> bool" where
-  "prepare_write svr t v s s' \<equiv>
-    prepare_write_G svr t v s \<and>
+definition prepare_write :: "key \<Rightarrow> txid0 \<Rightarrow> 'v \<Rightarrow> tstmp \<Rightarrow> ('v, 'm) global_conf_scheme \<Rightarrow> ('v, 'm) global_conf_scheme \<Rightarrow> bool" where
+  "prepare_write svr t v clk s s' \<equiv>
+    prepare_write_G svr t v clk s \<and>
     s' = prepare_write_U svr t v s"
 
 definition commit_write_G where
-  "commit_write_G svr t v cts s \<equiv>
+  "commit_write_G svr t v cts clk s \<equiv>
     is_curr_t s t \<and>
+    clk = Suc (max (svr_clock (svrs s svr)) (cl_clock (cls s (get_cl t)))) \<and>
     (\<exists>kv_map. cl_state (cls s (get_cl t)) = WtxnCommit cts kv_map \<and> svr \<in> dom kv_map) \<and>
     (\<exists>ts. svr_state (svrs s svr) (Tn t) = Prep ts v)"
 
@@ -468,9 +497,9 @@ definition commit_write_U where
       \<rparr>)
     \<rparr>"
 
-definition commit_write :: "key \<Rightarrow> txid0 \<Rightarrow> 'v \<Rightarrow> tstmp \<Rightarrow> ('v, 'm) global_conf_scheme \<Rightarrow> ('v, 'm) global_conf_scheme \<Rightarrow> bool" where
-  "commit_write svr t v cts s s' \<equiv>
-    commit_write_G svr t v cts s \<and>
+definition commit_write :: "key \<Rightarrow> txid0 \<Rightarrow> 'v \<Rightarrow> tstmp \<Rightarrow> tstmp \<Rightarrow> ('v, 'm) global_conf_scheme \<Rightarrow> ('v, 'm) global_conf_scheme \<Rightarrow> bool" where
+  "commit_write svr t v cts clk s s' \<equiv>
+    commit_write_G svr t v cts clk s \<and>
     s' = commit_write_U svr t v cts s"
 
 
@@ -492,16 +521,16 @@ definition state_init :: "'v global_conf" where
   \<rparr>"
 
 fun state_trans :: "('v, 'm) global_conf_scheme \<Rightarrow> 'v ev \<Rightarrow> ('v, 'm) global_conf_scheme \<Rightarrow> bool" where
-  "state_trans s (RInvoke cl keys sn)           s' \<longleftrightarrow> read_invoke cl keys sn s s'" |
-  "state_trans s (Read cl k v t rts rlst sn)    s' \<longleftrightarrow> read cl k v t rts rlst sn s s'" |
-  "state_trans s (RDone cl kv_map sn u'')       s' \<longleftrightarrow> read_done cl kv_map sn u'' s s'" |
-  "state_trans s (WInvoke cl kv_map sn)         s' \<longleftrightarrow> write_invoke cl kv_map sn s s'" |
-  "state_trans s (WCommit cl kv_map cts sn u'') s' \<longleftrightarrow> write_commit cl kv_map cts sn u'' s s'" |
-  "state_trans s (WDone cl kv_map sn)           s' \<longleftrightarrow> write_done cl kv_map sn s s'" |
-  "state_trans s (RegR svr t t_wr rts)          s' \<longleftrightarrow> register_read svr t t_wr rts s s'" |
-  "state_trans s (PrepW svr t v)                s' \<longleftrightarrow> prepare_write svr t v s s'" |
-  "state_trans s (CommitW svr t v cts)          s' \<longleftrightarrow> commit_write svr t v cts s s'" |
-  "state_trans s Skip2                          s' \<longleftrightarrow> s' = s"
+  "state_trans s (RInvoke cl keys sn clk)           s' \<longleftrightarrow> read_invoke cl keys sn clk s s'" |
+  "state_trans s (Read cl k v t rts rlst sn clk)    s' \<longleftrightarrow> read cl k v t rts rlst sn clk s s'" |
+  "state_trans s (RDone cl kv_map sn u'' clk)       s' \<longleftrightarrow> read_done cl kv_map sn u'' clk s s'" |
+  "state_trans s (WInvoke cl kv_map sn clk)         s' \<longleftrightarrow> write_invoke cl kv_map sn clk s s'" |
+  "state_trans s (WCommit cl kv_map cts sn u'' clk) s' \<longleftrightarrow> write_commit cl kv_map cts sn u'' clk s s'" |
+  "state_trans s (WDone cl kv_map sn clk)           s' \<longleftrightarrow> write_done cl kv_map sn clk s s'" |
+  "state_trans s (RegR svr t t_wr rts clk)          s' \<longleftrightarrow> register_read svr t t_wr rts clk s s'" |
+  "state_trans s (PrepW svr t v clk)                s' \<longleftrightarrow> prepare_write svr t v clk s s'" |
+  "state_trans s (CommitW svr t v cts clk)          s' \<longleftrightarrow> commit_write svr t v cts clk s s'" |
+  "state_trans s Skip2                              s' \<longleftrightarrow> s' = s"
 
 definition tps :: "('v ev, 'v global_conf) ES" where
   "tps \<equiv> \<lparr>
@@ -519,7 +548,7 @@ lemmas tps_trans_GU_defs =
   read_done_G_def read_done_U_def
   write_invoke_G_def write_invoke_U_def
   write_commit_G_def write_commit_U_def
-  write_done_G_def write_done_U_def
+  write_done_G_def clk_WDone_def write_done_U_def
   register_read_G_def register_read_U_def
   prepare_write_G_def prepare_write_U_def
   commit_write_G_def commit_write_U_def
